new/golang/theory/builtin.v
@@ -15,84 +15,55 @@ Section wps.
 
 Context `{sem: ffi_semantics} `{!ffi_interp ffi} `{!heapGS Σ}.
 
-Global Instance wp_int64_ge0 (x : w64) : PureWp True (int_ge0 #x) #(bool_decide (0 ≤ sint.Z x)).
-Proof.
-  pure_wp_start.
-  iExactEq "HΦ".
-  repeat f_equal.
-  apply bool_decide_ext.
-  word.
-Qed.
-
-(* NOTE: turned out to be unused *)
-Lemma swrap_neg (l: w64) :
-  sint.Z l < 0 →
-  word.swrap (word:=w64_word_instance) (uint.Z l) = uint.Z l - 2^64.
-Proof.
-  intros Hneg.
-  rewrite swrap_large; try word.
-Qed.
-
 Global Instance wp_int64_lt (l r : w64) : PureWp True (int_lt #l #r) #(bool_decide (sint.Z l < sint.Z r)).
-Proof.
-  pure_wp_start.
-  destruct (bool_decide_reflect (0 ≤ sint.Z l)%Z); wp_pures.
-  - destruct (bool_decide_reflect (0 ≤ sint.Z r)%Z); wp_pures.
-    + iExactEq "HΦ"; repeat f_equal; apply bool_decide_ext.
-      word.
-    + rewrite bool_decide_eq_false_2 //. word.
-  - destruct (bool_decide_reflect (0 ≤ sint.Z r)%Z); wp_pures.
-    + rewrite bool_decide_eq_true_2 //. word.
-    + iExactEq "HΦ"; repeat f_equal; apply bool_decide_ext.
-      word.
-Qed.
-
+Proof. by pure_wp_start. Qed.
 Global Instance wp_int64_gt (l r : w64) : PureWp True (int_gt #l #r) #(bool_decide (sint.Z l > sint.Z r)).
-Proof.
-  pure_wp_start.
-  iExactEq "HΦ"; repeat f_equal; apply bool_decide_ext.
-  word.
-Qed.
-
-Global Instance wp_int32_gt (l r : w32) : PureWp True (int_gt #l #r) #(bool_decide (sint.Z l > sint.Z r)).
-Proof. Admitted.
+Proof. pure_wp_start. repeat case_bool_decide; (done || lia). Qed.
+Global Instance wp_int64_leq (l r : w64) : PureWp True (int_leq #l #r) #(bool_decide (sint.Z l ≤ sint.Z r)).
+Proof. by pure_wp_start. Qed.
+Global Instance wp_int64_geq (l r : w64) : PureWp True (int_geq #l #r) #(bool_decide (sint.Z l >= sint.Z r)).
+Proof. pure_wp_start. repeat case_bool_decide; (done || lia). Qed.
 
 Global Instance wp_int32_lt (l r : w32) : PureWp True (int_lt #l #r) #(bool_decide (sint.Z l < sint.Z r)).
-Proof. Admitted.
-
-Global Instance wp_int64_leq (l r : w64) : PureWp True (int_leq #l #r) #(bool_decide (sint.Z l ≤ sint.Z r)).
-Proof.
-  pure_wp_start.
-  destruct (bool_decide_reflect (l = r)); wp_pures.
-  - rewrite bool_decide_eq_true_2 //. word.
-  - iExactEq "HΦ"; repeat f_equal; apply bool_decide_ext.
-    word.
-Qed.
-
-Global Instance wp_int64_geq (l r : w64) : PureWp True (int_geq #l #r) #(bool_decide (sint.Z l >= sint.Z r)).
-Proof.
-  pure_wp_start.
-  iExactEq "HΦ"; repeat f_equal; apply bool_decide_ext.
-  word.
-Qed.
-
-Global Instance wp_int32_geq (l r : w32) : PureWp True (int_geq #l #r) #(bool_decide (sint.Z l >= sint.Z r)).
-Proof. Admitted.
-
+Proof. by pure_wp_start. Qed.
+Global Instance wp_int32_gt (l r : w32) : PureWp True (int_gt #l #r) #(bool_decide (sint.Z l > sint.Z r)).
+Proof. pure_wp_start. repeat case_bool_decide; (done || lia). Qed.
 Global Instance wp_int32_leq (l r : w32) : PureWp True (int_leq #l #r) #(bool_decide (sint.Z l ≤ sint.Z r)).
-Proof. Admitted.
+Proof. by pure_wp_start. Qed.
+Global Instance wp_int32_geq (l r : w32) : PureWp True (int_geq #l #r) #(bool_decide (sint.Z l >= sint.Z r)).
+Proof. pure_wp_start. repeat case_bool_decide; (done || lia). Qed.
+
+Global Instance wp_int16_lt (l r : w16) : PureWp True (int_lt #l #r) #(bool_decide (sint.Z l < sint.Z r)).
+Proof. by pure_wp_start. Qed.
+Global Instance wp_int16_gt (l r : w16) : PureWp True (int_gt #l #r) #(bool_decide (sint.Z l > sint.Z r)).
+Proof. pure_wp_start. repeat case_bool_decide; (done || lia). Qed.
+Global Instance wp_int16_leq (l r : w16) : PureWp True (int_leq #l #r) #(bool_decide (sint.Z l ≤ sint.Z r)).
+Proof. by pure_wp_start. Qed.
+Global Instance wp_int16_geq (l r : w16) : PureWp True (int_geq #l #r) #(bool_decide (sint.Z l >= sint.Z r)).
+Proof. pure_wp_start. repeat case_bool_decide; (done || lia). Qed.
+
+Global Instance wp_int8_lt (l r : w8) : PureWp True (int_lt #l #r) #(bool_decide (sint.Z l < sint.Z r)).
+Proof. by pure_wp_start. Qed.
+Global Instance wp_int8_gt (l r : w8) : PureWp True (int_gt #l #r) #(bool_decide (sint.Z l > sint.Z r)).
+Proof. pure_wp_start. repeat case_bool_decide; (done || lia). Qed.
+Global Instance wp_int8_leq (l r : w8) : PureWp True (int_leq #l #r) #(bool_decide (sint.Z l ≤ sint.Z r)).
+Proof. by pure_wp_start. Qed.
+Global Instance wp_int8_geq (l r : w8) : PureWp True (int_geq #l #r) #(bool_decide (sint.Z l >= sint.Z r)).
+Proof. pure_wp_start. repeat case_bool_decide; (done || lia). Qed.
 
 Lemma wp_make_nondet_uint64 (v : val) :
   {{{ True }}}
-    make_nondet uint64T v
+    make_nondet go.uint64 v
   {{{ (x : w64), RET #x; True }}}.
 Proof.
-  iIntros (?) "_ HΦ". wp_call. wp_apply wp_ArbitraryInt. rewrite to_val_unseal //.
+  iIntros (?) "_ HΦ". wp_call. rewrite decide_True //. wp_apply wp_ArbitraryInt.
+  rewrite to_val_unseal //.
 Qed.
 
+(*
 Lemma wp_make_nondet_float64 (v : val) :
   {{{ True }}}
-    make_nondet float64T v
+    make_nondet go.float64T v
   {{{ (x : w64), RET #x; True }}}.
 Proof.
   apply wp_make_nondet_uint64.
@@ -115,7 +86,7 @@ Lemma wp_make_nondet_float32 (v : val) :
   {{{ (x : w32), RET #x; True }}}.
 Proof.
   apply wp_make_nondet_uint32.
-Qed.
+Qed. *)
 
 End wps.
 
